Intermediate/Decomposition.v
@@ -12,6 +12,13 @@ Require Import S2I.Definitions.
 
 Import Intermediate.
 
+Ltac simplify_turn :=
+  unfold S.PS.is_program_component, S.PS.is_context_component in *;
+  unfold I.PS.is_program_component, I.PS.is_context_component in *;
+  unfold turn_of, S.PS.state_turn, I.PS.state_turn in *;
+  simpl in *;
+  auto.
+
 Section Decomposition.
   Variable prog: Intermediate.program.
   Variable ctx: Program.interface.
@@ -19,10 +26,10 @@ Section Decomposition.
   (*
   Hypothesis input_program_closedness:
     Intermediate.closed_program prog.
+   *)
 
   Hypothesis context_validity:
     forall C CI, PMap.MapsTo C CI ctx -> PMap.MapsTo C CI (Intermediate.prog_interface prog).
-  *)
 
   Let G : Intermediate.GlobalEnv.global_env := Intermediate.GlobalEnv.init_genv prog.
 
@@ -33,8 +40,40 @@ Section Decomposition.
       I.PS.initial_state prog ctx ips /\ I.PS.partial_state ctx ics ips.
   Proof.
     intros ics Hics_init.
+    I.CS.unfold_state.
     (* case analysis on who has control, then build the partial state *)
-  Admitted.
+    destruct (PMap.mem (Pointer.component pc) ctx) eqn:Htarget.
+    (* context has control *)
+    - exists (I.PS.CC (Pointer.component pc,
+                  I.PS.to_partial_stack s (map fst (PMap.elements ctx)),
+                  PMapExtra.filter (fun k _ => negb (PMap.mem k ctx)) mem) Normal).
+      split.
+      + econstructor.
+        * eapply I.PS.ContextControl_Normal; eauto.
+          ** simplify_turn.
+             apply PMapFacts.mem_in_iff. auto.
+          ** apply PMapFacts.Equal_refl.
+        * eauto.
+      + eapply I.PS.ContextControl_Normal; eauto.
+          ** simplify_turn.
+             apply PMapFacts.mem_in_iff. auto.
+          ** apply PMapFacts.Equal_refl.
+    (* program has control *)
+    - exists (I.PS.PC (I.PS.to_partial_stack s (map fst (PMap.elements ctx)),
+                  PMapExtra.filter (fun k _ => negb (PMap.mem k ctx)) mem,
+                  regs, pc)).
+      split.
+      + econstructor.
+        * eapply I.PS.ProgramControl; auto.
+          ** simplify_turn.
+             apply PMapFacts.not_mem_in_iff. auto.
+          ** apply PMapFacts.Equal_refl.
+        * eauto.
+      + eapply I.PS.ProgramControl; auto.
+          ** simplify_turn.
+             apply PMapFacts.not_mem_in_iff. auto.
+          ** apply PMapFacts.Equal_refl.
+  Qed.
 
   Lemma match_final_states:
     forall ics ips r,
@@ -43,15 +82,98 @@ Section Decomposition.
       I.PS.final_state prog ctx ips r.
   Proof.
     intros ics ips r Hpartial Hics_final.
+    I.CS.unfold_state.
     (* case analysis on who has control *)
-  Admitted.
+    destruct (PMap.mem (Pointer.component pc) ctx) eqn:Htarget.
+    (* context has control *)
+    - inversion Hpartial; inversion H; subst.
+      + simplify_turn.
+        apply PMapFacts.mem_in_iff in Htarget.
+        contradiction.
+      + apply I.PS.final_state_context.
+        simplify_turn.
+    (* program has control *)
+    - inversion Hpartial; inversion H; subst.
+      + eapply I.PS.final_state_program.
+        * simplify_turn.
+        * eauto.
+        * eauto.
+      + apply PMapFacts.not_mem_in_iff in Htarget.
+        contradiction.
+  Qed.
 
-  Ltac simplify_turn :=
-    unfold S.PS.is_program_component, S.PS.is_context_component in *;
-    unfold I.PS.is_program_component, I.PS.is_context_component in *;
-    unfold turn_of, S.PS.state_turn, I.PS.state_turn in *;
-    simpl in *;
-    auto.
+  Lemma pc_inc_within_partial_frame_1:
+    forall pc,
+      PMap.In (Pointer.component pc) ctx ->
+      I.PS.to_partial_frame (map fst (PMap.elements ctx)) pc = (Pointer.component pc, None).
+  Proof.
+    intros pc Hin_ctx.
+    unfold I.PS.to_partial_frame, Pointer.inc, Pointer.add.
+    destruct pc as [[C b] o].
+    simpl in *. simplify_turn.
+    destruct (Util.Lists.mem C (map fst (PMap.elements ctx))) eqn:Hin.
+    *** reflexivity.
+    *** exfalso. (* contra *)
+        apply Util.Lists.not_in_iff_mem_false in Hin.
+        apply Hin.
+        unfold PMap.In, PMap.Raw.In0 in Hin_ctx.
+        destruct Hin_ctx as [CI HCI].
+        apply PMapFacts.elements_mapsto_iff in HCI.
+        apply SetoidList.InA_altdef in HCI.
+        apply Exists_exists in HCI.
+        destruct HCI as [[] []].
+        apply in_map_iff. exists (k,i). simpl. split.
+        **** inversion H0. inversion H1. auto.
+        **** auto.
+  Qed.
+
+  Lemma pc_inc_within_partial_frame_2:
+    forall pc,
+      ~ PMap.In (Pointer.component pc) ctx ->
+      I.PS.to_partial_frame (map fst (PMap.elements ctx)) pc
+      = (Pointer.component pc, Some (Pointer.block pc, Pointer.offset pc)).
+  Proof.
+    intros pc Hnot_in_ctx.
+    unfold I.PS.to_partial_frame, Pointer.inc, Pointer.add.
+    destruct pc as [[C b] o].
+    simpl in *. simplify_turn.
+    destruct (Util.Lists.mem C (map fst (PMap.elements ctx))) eqn:Hin.
+    *** exfalso. (* contra *)
+        apply Util.Lists.in_iff_mem_true in Hin.
+        apply Hnot_in_ctx. unfold PMap.In, PMap.Raw.In0.
+        apply in_map_iff in Hin. destruct Hin as [[] []].
+        simpl in *. subst.
+        eexists.
+        apply PMapFacts.elements_mapsto_iff.
+        apply SetoidList.In_InA.
+        **** econstructor.
+             ***** constructor; reflexivity.
+             ***** constructor; destruct x; destruct y; inversion H; auto.
+             ***** constructor; destruct x; destruct y; destruct z;
+                   inversion H; inversion H1; simpl in *; subst; auto.
+        **** apply H0.
+    *** reflexivity.
+  Qed.
+
+  Lemma imported_procedure_in_context:
+    forall C C' P,
+      PMap.In C ctx ->
+      imported_procedure (genv_interface G) C C' P ->
+      imported_procedure ctx C C' P.
+  Proof.
+    intros C C' P Hin_ctx Himport.
+    unfold imported_procedure in *.
+    unfold PMap.In, PMap.Raw.In0 in Hin_ctx.
+    destruct Hin_ctx as [CI HCI].
+    destruct Himport as [CI' [HCI' Himp]].
+    unfold Program.has_component in *.
+    assert (HCI2 := HCI).
+    apply context_validity in HCI.
+    unfold G, init_genv in HCI'.
+    destruct (init_all prog). destruct p. simpl in *.
+    pose proof (PMapFacts.MapsTo_fun HCI HCI'). subst.
+    exists CI'. split; auto.
+  Qed.
 
   Lemma lockstep_simulation:
     forall ics t ics',
@@ -137,18 +259,80 @@ Section Decomposition.
         ** simplify_turn.
            unfold Pointer.inc, Pointer.add. destruct pc. destruct p. auto.
 
-    - eexists. split.
-      + econstructor; auto.
-        * apply Hstep.
+    - destruct (Memory.store pmem ptr (Register.get r2 regs)) as [pmem'|] eqn:Hpmem'.
+      + exists (I.PS.PC (I.PS.to_partial_stack gps (map fst (PMap.elements ctx)),
+                    pmem', regs, Pointer.inc pc)).
+        split.
         * econstructor; auto.
+          ** apply Hstep.
+          ** econstructor; auto.
+          ** econstructor; eauto.
+             *** simplify_turn.
+                 unfold Pointer.inc, Pointer.add. destruct pc. destruct p. auto.
+             *** unfold Memory.store in *.
+                 destruct ptr; destruct p.
+                 destruct (PMap.find i pmem)
+                          eqn:Hmem_find1; try discriminate.
+                 destruct (ComponentMemory.store t i0 o (Register.get r2 regs))
+                          eqn:Hmem_store1; try discriminate.
+                 inversion Hpmem'; subst.
+                 destruct (PMap.find i mem)
+                   eqn:Hmem_find2; try discriminate.
+                 destruct (ComponentMemory.store t1 i0 o (Register.get r2 regs))
+                   eqn:Hmem_store2; try discriminate.
+                 inversion H10; subst.
+                 assert (t = t1). {
+                   specialize (H2 i). rewrite H2 in Hmem_find1.
+                   apply PMapFacts.find_mapsto_iff in Hmem_find1.
+                   apply PMapExtra.filter_iff in Hmem_find1.
+                   destruct Hmem_find1.
+                   apply PMap.find_1 in H. rewrite H in Hmem_find2.
+                   inversion Hmem_find2. reflexivity.
+                   (* morphisms stuff *)
+                   unfold Morphisms.Proper, Morphisms.respectful.
+                   intros. subst. reflexivity.
+                 }
+                 subst.
+                 rewrite Hmem_store2 in Hmem_store1. inversion Hmem_store1.
+                 subst.
+                 rewrite H2.
+
+                 unfold PMap.Equal. intro.
+                 rewrite PMapFacts.add_o.
+                 destruct (PMapFacts.eq_dec i y).
+                 **** subst. admit.
+                 **** admit.
         * econstructor; eauto.
           ** simplify_turn.
              unfold Pointer.inc, Pointer.add. destruct pc. destruct p. auto.
           ** admit.
-      + econstructor; auto.
-        ** simplify_turn.
-           unfold Pointer.inc, Pointer.add. destruct pc. destruct p. auto.
-        ** admit.
+      + (* contra *)
+        unfold Memory.store in *.
+        destruct ptr; destruct p.
+        destruct (PMap.find i mem)
+                 eqn:Hmem_find2; try discriminate.
+        destruct (ComponentMemory.store t i0 o (Register.get r2 regs))
+                 eqn:Hmem_store1; try discriminate.
+        inversion H10; subst.
+        destruct (PMap.find i pmem)
+                 eqn:Hmem_find1; try discriminate.
+        * destruct (ComponentMemory.store t1 i0 o (Register.get r2 regs))
+                 eqn:Hmem_store2; try discriminate.
+          assert (t = t1). {
+            specialize (H2 i). rewrite H2 in Hmem_find1.
+            apply PMapFacts.find_mapsto_iff in Hmem_find1.
+            apply PMapExtra.filter_iff in Hmem_find1.
+            destruct Hmem_find1.
+            apply PMap.find_1 in H. rewrite H in Hmem_find2.
+            inversion Hmem_find2. reflexivity.
+            (* morphisms stuff *)
+            unfold Morphisms.Proper, Morphisms.respectful.
+            intros. subst. reflexivity.
+          }
+          subst.
+          rewrite Hmem_store2 in Hmem_store1. inversion Hmem_store1.
+        * (* contra *)
+          admit.
 
     - eexists. split.
       + econstructor; auto.
@@ -195,19 +379,71 @@ Section Decomposition.
         * econstructor; eauto.
           ** simplify_turn.
              unfold Pointer.inc, Pointer.add. destruct pc. destruct p. auto.
-          ** admit.
+          ** (* should be provable *) admit.
       + econstructor; auto.
-          ** simplify_turn.
-             unfold Pointer.inc, Pointer.add. destruct pc. destruct p. auto.
-          ** admit.
+        ** simplify_turn.
+           unfold Pointer.inc, Pointer.add. destruct pc. destruct p. auto.
+        ** (* should be provable *) admit.
 
     (* call *)
-    - (* case analysis on the target *)
-      admit.
+    (* case analysis on the target *)
+    - destruct (PMap.mem C' ctx) eqn:Htarget.
+      (* external call *)
+      + eexists. split.
+        * eapply I.PS.Program_External_Call; eauto.
+          ** reflexivity.
+          ** simplify_turn.
+             apply PMapFacts.mem_in_iff. auto.
+        * eapply I.PS.ContextControl_Normal; eauto.
+          ** simplify_turn.
+             apply PMapFacts.mem_in_iff. auto.
+          ** unfold I.PS.to_partial_stack. simpl.
+             rewrite pc_inc_within_partial_frame_2; auto.
+             unfold Pointer.inc, Pointer.add. destruct pc as [[]]. reflexivity.
+             unfold Pointer.inc, Pointer.add. destruct pc as [[]]. simpl. simplify_turn.
+      (* internal call *)
+      + eexists. split.
+        * eapply I.PS.Program_Internal_Call; eauto.
+          ** reflexivity.
+          ** simplify_turn.
+             apply PMapFacts.not_mem_in_iff. auto.
+        * eapply I.PS.ProgramControl; eauto.
+          ** simplify_turn.
+             apply PMapFacts.not_mem_in_iff. auto.
+          ** unfold I.PS.to_partial_stack. simpl.
+             rewrite pc_inc_within_partial_frame_2; auto.
+             unfold Pointer.inc, Pointer.add. destruct pc as [[]]. reflexivity.
+             unfold Pointer.inc, Pointer.add. destruct pc as [[]]. simpl. simplify_turn.
 
     (* return *)
-    - (* case analysis on the target *)
-      admit.
+    (* case analysis on the target *)
+    - destruct (PMap.mem (Pointer.component pc') ctx) eqn:Htarget.
+      (* external return *)
+      + eexists. split.
+        * eapply I.PS.Program_External_Return; eauto.
+          ** reflexivity.
+          ** simplify_turn.
+             apply PMapFacts.mem_in_iff. auto.
+          ** unfold I.PS.to_partial_stack. simpl.
+             apply PMapFacts.mem_in_iff in Htarget.
+             rewrite pc_inc_within_partial_frame_1; auto.
+        * eapply I.PS.ContextControl_Normal; eauto.
+          ** simplify_turn.
+             apply PMapFacts.mem_in_iff. auto.
+      (* internal return *)
+      + eexists. split.
+        * eapply I.PS.Program_Internal_Return; eauto.
+          ** reflexivity.
+          ** simplify_turn.
+             apply PMapFacts.not_mem_in_iff. auto.
+          ** unfold I.PS.to_partial_stack. simpl.
+             rewrite pc_inc_within_partial_frame_2.
+             *** reflexivity.
+             *** apply PMapFacts.not_mem_in_iff. auto.
+        * eapply I.PS.ProgramControl; eauto.
+          ** destruct pc' as [[]]. simpl. reflexivity.
+          ** simplify_turn.
+             apply PMapFacts.not_mem_in_iff. auto.
 
     (** context has control **)
 
@@ -246,7 +482,7 @@ Section Decomposition.
       + eapply I.PS.Context_Epsilon; auto.
       + eapply I.PS.ContextControl_Normal; eauto.
         * unfold Pointer.inc, Pointer.add. destruct pc. destruct p. reflexivity.
-        * admit.
+        * (* should be provable *) admit.
 
     - eexists. split.
       + eapply I.PS.Context_Epsilon; auto.
@@ -272,15 +508,121 @@ Section Decomposition.
       + eapply I.PS.Context_Epsilon; auto.
       + eapply I.PS.ContextControl_Normal; eauto.
         * unfold Pointer.inc, Pointer.add. destruct pc. destruct p. reflexivity.
-        * admit.
+        * (* should be provable *) admit.
 
     (* call *)
-    - (* case analysis on the target *)
-      admit.
+    (* case analysis on the target *)
+    - destruct (PMap.mem C' ctx) eqn:Htarget.
+      (* internal call *)
+      + eexists. split.
+        * eapply I.PS.Context_Internal_Call.
+          ** eauto.
+          ** eauto.
+          ** reflexivity.
+          ** simplify_turn.
+          ** simplify_turn.
+             apply PMapFacts.mem_in_iff. auto.
+          ** auto.
+          ** simplify_turn.
+             apply imported_procedure_in_context; auto.
+          ** eauto.
+        * eapply I.PS.ContextControl_Normal.
+          ** eauto.
+          ** eauto.
+          ** simplify_turn.
+             apply PMapFacts.mem_in_iff. auto.
+          ** auto.
+          ** unfold I.PS.to_partial_stack. simpl.
+             apply PMapFacts.mem_in_iff in Htarget.
+             rewrite pc_inc_within_partial_frame_1.
+             *** unfold Pointer.inc, Pointer.add.
+                 destruct pc as [[]]. reflexivity.
+             *** unfold Pointer.inc, Pointer.add.
+                 destruct pc as [[]]. simpl. simplify_turn.
+      (* external call *)
+      + exists (I.PS.PC ((Pointer.component pc, None) ::
+                    I.PS.to_partial_stack gps (map fst (PMap.elements ctx)),
+                    pmem, Register.invalidate regs, pc')).
+        split.
+        * eapply I.PS.Context_External_Call.
+          ** eauto.
+          ** eauto.
+          ** reflexivity.
+          ** simplify_turn.
+          ** simplify_turn.
+             apply PMapFacts.not_mem_in_iff.
+             change C' with (Pointer.component pc') in Htarget.
+             apply Htarget.
+          ** simplify_turn.
+             apply imported_procedure_in_context; auto.
+          ** eauto.
+          ** eauto.
+          ** eauto.
+          ** eauto.
+        * eapply I.PS.ProgramControl; auto.
+          ** simplify_turn.
+             apply PMapFacts.not_mem_in_iff. auto.
+          ** unfold I.PS.to_partial_stack. simpl.
+             rewrite pc_inc_within_partial_frame_1.
+             *** unfold Pointer.inc, Pointer.add.
+                 destruct pc as [[]]. reflexivity.
+             *** unfold Pointer.inc, Pointer.add.
+                 destruct pc as [[]]. simpl. simplify_turn.
 
     (* return *)
-    - (* case analysis on the target *)
-      admit.
+    (* case analysis on the target *)
+    - destruct (PMap.mem (Pointer.component pc') ctx) eqn:Htarget.
+      (* internal return *)
+      + eexists. split.
+        * eapply I.PS.Context_Internal_Return.
+          ** eauto.
+          ** eauto.
+          ** reflexivity.
+          ** simplify_turn.
+          ** simplify_turn.
+             apply PMapFacts.mem_in_iff. auto.
+          ** auto.
+          ** unfold I.PS.to_partial_stack. simpl.
+             apply PMapFacts.mem_in_iff in Htarget.
+             rewrite pc_inc_within_partial_frame_1.
+             *** unfold Pointer.inc, Pointer.add.
+                 destruct pc as [[]]. reflexivity.
+             *** unfold Pointer.inc, Pointer.add.
+                 destruct pc as [[]]. simpl. simplify_turn.
+        * eapply I.PS.ContextControl_Normal.
+          ** eauto.
+          ** eauto.
+          ** simplify_turn.
+             apply PMapFacts.mem_in_iff. auto.
+          ** auto.
+          ** eauto.
+      (* external return *)
+      + exists (I.PS.PC (I.PS.to_partial_stack gps' (map fst (PMap.elements ctx)),
+                    pmem, Register.invalidate regs, pc')).
+        split.
+        * eapply I.PS.Context_External_Return.
+          ** eauto.
+          ** eauto.
+          ** reflexivity.
+          ** simplify_turn.
+          ** simplify_turn.
+             apply PMapFacts.not_mem_in_iff. eauto.
+          ** eauto.
+          ** unfold I.PS.to_partial_stack. simpl.
+             apply PMapFacts.not_mem_in_iff in Htarget.
+             rewrite pc_inc_within_partial_frame_2.
+             *** unfold Pointer.inc, Pointer.add.
+                 destruct pc as [[]]. reflexivity.
+             *** unfold Pointer.inc, Pointer.add.
+                 destruct pc as [[]]. simpl. simplify_turn.
+          ** destruct pc' as [[]]. reflexivity.
+        * eapply I.PS.ProgramControl.
+          ** eauto.
+          ** reflexivity.
+          ** simplify_turn.
+             apply PMapFacts.not_mem_in_iff. auto.
+          ** eauto.
+          ** auto.
   Admitted.
 
   Theorem decomposition:
@@ -310,8 +652,11 @@ Section DecompositionAndLinking.
   Corollary decomposition_with_linking:    
     forward_simulation (I.CS.sem (Intermediate.program_link p c mainC mainP))
                        (I.PS.sem (Intermediate.program_link p c mainC mainP)
-                                 (Intermediate.prog_interface p)).
+                                 (Intermediate.prog_interface c)).
   Proof.
     apply decomposition.
+    intros C CI Hin_c.
+    unfold program_link. simpl.
+    apply PMapExtra.update_mapsto_iff. left. auto.
   Qed.
 End DecompositionAndLinking.
